implement IsVerifiedQuorum transition for LH_HANDSHAKE_A

ironfleet/src/Dafny/Distributed/Protocol/ZooKeeper/LearnerHandler.dfy
@@ -9,29 +9,56 @@ import opened ZooKeeper_ZKDatabase
 import opened ZooKeeper_Environment
 
 
+datatype LearnerHandlerState = LH_HANDSHAKE_A | LH_HANDSHAKE_B | LH_DECIDE_SYNC | LH_SYNC | LH_RUNNING | LH_ERROR
+/*
+* LH_HANDSHAKE_A: Receive FOLLOWERINFO, wait for quorum, then send new epoch
+* LH_HANDSHAKE_B: Wait for a quorum of ACKEPOCH response. This ends the handshake with follower
+* LH_DECIDE_SYNC: 
+*/
+
+
 // config[my_id] is my own endpoint, config[follower_id] is the follower endpoint
 datatype LearnerHandler = LearnerHandler(
     my_id: nat,
     follower_id: nat,
     config: Config,
     zkdb: ZKDatabase,  //This is the leader db, and is not specified by LearnerHandler
-    state: LearnerHandlerState 
+    state: LearnerHandlerState,
+    globals: LeaderGlobals,
+
+    // Local state
+    newEpoch: int
 )
 
-datatype LearnerHandlerState = LH_HANDSHAKE_A | LH_HANDSHAKE_B | LH_DECIDE_SYNC | LH_SYNC | LH_RUNNING | LH_ERROR
+
+/* Global Leader variables shared by all LearnerHandler threads */
+datatype LeaderGlobals = LearnerHandler(
+    zkdb: ZKDatabase,
+
+    // Handshake globals
+    leaderEpoch: int,
+    connectingFollowers: set<nat>
+)
 
 
-predicate LearnerHandlerInit(s:LearnerHandler, my_id:nat, follower_id:nat, config:Config, zkdb: ZKDatabase) {
+/*****************************************************************************************
+*                                      Actions                                           *
+******************************************************************************************/ 
+
+predicate LearnerHandlerInit(s:LearnerHandler, my_id:nat, follower_id:nat, config:Config, zkdb: ZKDatabase, globals: LeaderGlobals) {
     && s.my_id == my_id
-    && s.follower_id == follower_id
+    && s.follower_id == s.follower_id  // follower id is initially unknown
     && s.config == config
     && s.zkdb == zkdb
     && s.state == LH_HANDSHAKE_A
+    && s.globals == globals
+
+    && s.newEpoch == -1
 }
 
 predicate LearnerHandlerNext(s:LearnerHandler, s':LearnerHandler, ios:seq<ZKIo>) {
     match s.state 
-        case LH_HANDSHAKE_A => false
+        case LH_HANDSHAKE_A => GetEpochToPropose(s, s', ios)
         case LH_HANDSHAKE_B => false
         case LH_DECIDE_SYNC => false
         case LH_SYNC => false
@@ -43,4 +70,44 @@ predicate LearnerHandlerStutter(s:LearnerHandler, s':LearnerHandler) {
     s' == s
 }
 
+predicate GetEpochToPropose(s:LearnerHandler, s':LearnerHandler, ios:seq<ZKIo>) {
+    if IsVerifiedQuorum(s.my_id, |s.config|, s.globals.connectingFollowers) 
+    then (
+        // Send Leader.LEADERINFO message to follower, and proceed to LH_HANDSHAKE_B state
+        && |ios| == 1
+        && s' == s.(state := LH_HANDSHAKE_B, newEpoch := s.globals.leaderEpoch)
+        && ios[0].LIoOpSend?
+        && (var outbound_packet := ios[0].s;
+            && 0 <= s.follower_id < |s.config|
+            && outbound_packet.dst == s.config[s.follower_id]
+            && outbound_packet.msg == LeaderInfo(s.my_id, Zxid(s.globals.leaderEpoch, 0))
+        )       
+    ) else (
+        // Add sender to my connectingFollowers set, and continue waiting for quorum
+        if |ios| == 0 then LearnerHandlerStutter(s, s')  // Case where follower has not sent anything
+        else && |ios| == 1
+             && ios[0].LIoOpReceive?
+             && ios[0].r.src in s.config
+             && ios[0].r.msg.FollowerInfo?
+             && 0 <= ios[0].r.msg.sid < |s.config| 
+             && s.config[ios[0].r.msg.sid] == ios[0].r.src
+             && s' == s.(
+                 follower_id := ios[0].r.msg.sid,
+                 globals := s.globals.(
+                    leaderEpoch := (if ios[0].r.msg.latestZxid.epoch >= s.globals.leaderEpoch then ios[0].r.msg.latestZxid.epoch + 1 else s.globals.leaderEpoch),
+                    connectingFollowers := s.globals.connectingFollowers + {ios[0].r.msg.sid}
+                )
+             )
+    )
+}
+
+
+/*****************************************************************************************
+*                                    Helper defs                                         *
+******************************************************************************************/ 
+
+predicate IsVerifiedQuorum(my_id:nat, n:int, quorum: set<nat>) {
+    && my_id in quorum
+    && |quorum| >= (n/2) + 1
+}
 }
